---
title: "Lesson 5: Velocity Addition"
format: revealjs
title-slide-attributes:
  data-notes: ""
---

# Recap

## The Lorentz transform

$$
\begin{align*}
x'&=\gamma(x-vt)\\
t'&=\gamma\left(t-\frac{vx}{c^2}\right)\\
\\
x&=\gamma(x'+vt')\\
t&=\gamma\left(t'+\frac{vx'}{c^2}\right)
\end{align*}
$$

## The Lorentz transform

Or, with $\beta=\frac{v}{c}$ and using $ct,ct'$ instead of $t,t'$:
$$
\begin{align*}
x'&=\gamma(x-\beta ct)\\
ct'&=\gamma(ct-\beta x)\\
\\
x&=\gamma(x'+\beta ct')\\
ct&=\gamma(ct'+\beta x')
\end{align*}
$$

# Velocity addition

## Non-relativistic velocity addition

* Velocities of non-light objects “just add normally”: [add the velocity of the frame and the velocity of the object in the frame.]{.fragment}
	* If $A$ is traveling at $0.9c$ relative to $B$, and $A$ launches something forwards at $0.9c$ relative to $A$, $B$ would observe the speed of the object as $1.8c>c$.
* Yet the velocity of light is constant and universal: [it's $c$ in every frame.]{.fragment}
* This is weird, and bad, and wrong.

## Relativistic velocity addition

* What we'd hope for:
* Velocities of non-light objects add in a specific way, $v_\textrm{net}=f(v_\textrm{frame}, v_\textrm{object}')$.
* The velocity of light adds in _the same_ way, $c=f(v_\textrm{frame}, c)$.
* Note: now we have three frames: [our unprimed “stationary” frame,]{.fragment} [the primed “moving” frame,]{.fragment} [and the frame of the object moving in the primed frame!]{.fragment}

## Setup

* Primed frame $F'$ with origin $O'$ is moving in $F$ with velocity $v$.
* “Double-primed” frame $F''$ with origin $O''$ is moving in $F'$ with velocity $u'$.
* Q: What is the apparent velocity $u$ of $F''$ in $F$?

## Setup

![](/images/5/velo-add-1.svg){fig-align="center"}

## Setup

* We'll put a flashlight at $O''$.
* The flashlight emits a photon every $\Delta t''$ in its own frame (it's connected to a light clock with period $\Delta t''$).
* We will determine the period of photons arriving at $O'$ and then $O$.

## Setup

![](/images/5/velo-add-2.svg){fig-align="center"}

## Part 1: Rates of arrival

* In general (forget this particular setup): [If a blinking flashlight has period $T'$ and velocity $v$, then the period of photons arriving at us from the flashlight will be $f(v)T'$ for some $f$ that we need to find.]{.fragment}
* So the period of photons arriving at $O'$ will be $\Delta t'=f(u')\Delta t''$.

## Part 1: Rates of arrival

* Now consider the period of photons arriving at $O$.
	* On the one hand, $O''$ has apparent velocity $u'$, so the period will be $\Delta t=f(u)\Delta t''$.
	* On the other hand, the photons also pass through $O'$, which has speed $v$ and “emits” the photons with period $\Delta t'=f(u')\Delta t''$.
	* So $\Delta t=f(v)\Delta t''=f(v)f(u')\Delta t''$
	* And	therefore $f(u)=f(v)f(u')$!

* We have a relation between $u$, $v$, and $u'$. [Find $f$ and we're done(ish).]{.fragment}

## Part 2: Finding $f$

* Consider our blinking flashlight with velocity $v$ and period $T'$.
* With what period do we receive photons?
	* If the flashlight were stationary, the period would just be $T'$.
	* But it's moving, so

	   1. It is time dilated — to us, it emits a photon every $\gamma T'$.
      1. Each photon is emitted a distance $v\gamma T'$ from the previous one.

## Part 2: Finding $f$

* Each photon has to travel for an additional time $\frac{v\gamma T'}{c}=\gamma\beta T'$ than the previous to arrive at us (or less time if $v<0$).
* Each photon arrives at us a time $T=\gamma T'+ \gamma\beta T'=\gamma_{u'}(1+\beta_{u'})\Delta t''$ after the previous.
* Therefore, $f(v)=\gamma_v(1+\beta_v)$.

## Part 2: Finding $f$

* Let's simplify:

::: {.fragment}
$$
\begin{align*}
f(v)&\class{fragment}{{}=\gamma_{v}(1+\beta_{v})}\\
&\class{fragment}{{}=\frac{(1+\beta_{v})}{\sqrt{1-\beta_{v}^2}}}
\end{align*}
$$
:::

## Part 2: Finding $f$

$$
\begin{align*}
f(v)&=\frac{1+\beta_{v}}{\sqrt{1-\beta_{v}^2}}\\
&\class{fragment}{{}=\frac{(1+\beta_{v})}{\sqrt{(1-\beta_{v})(1+\beta_{v})}}}\\
&\class{fragment}{{}=\frac{\sqrt{1+\beta_{v}}}{\sqrt{1-\beta_{v}}}}\\
&\class{fragment}{{}=\sqrt{\frac{1+\beta_{v}}{1-\beta_{v}}}}
\end{align*}
$$

::: {.notes}
As expected, this is greater than 1 if beta>0. It's also less than 1 if beta<0, although this isn't as obvious from the outset.
:::

## Part 2

* Now, consider the photons as they reach $O$.
	* They were emitted by $F''$, so they arrive with period $f(u)\Delta t''$
	* And they passed

* Suppose that $F'$ emits a photon towards $O$ whenever a photon arrives at $O'$. [$O'$ is now effectively the same kind of flashlight in $F$ as the actual flashlight was in $F'$.]{.fragment}
* If $F'$ emits flashes with period $\Delta t'$ in its frame, then $F$ perceives them arrive with period $\Delta t_\textrm{arr}=\Delta t'\sqrt{\frac{1-\beta_v}{1+\beta_v}}$.
* But we know that in fact $\Delta t'=\Delta t'_\textrm{arr}=\Delta t''\sqrt{\frac{1+\beta_{u'}}{1-\beta_{u'}}}$
* Result: the flashes arrive at $O$ with period $\Delta t_\textrm{arr}=\Delta t''\sqrt{\frac{1+\beta_{u'}}{1-\beta_{u'}}}\sqrt{\frac{1+\beta_v}{1-\beta_v}}$.

## Part 3

* Key point: [$F'$ emitting a photon whenever it receives one is _identical_ to the original photon just passing through $O'$!]{.fragment}
* That is, $O$ receives flashes _from the flashlight_ with period $\Delta t_\textrm{arr}=\Delta t''\sqrt{\frac{1+\beta_{u'}}{1-\beta_{u'}}}\sqrt{\frac{1+\beta_v}{1-\beta_v}}$.
* But the flashlight is also moving in $F$, and we know the period shift of moving flashlights based on their velocity...
	* It's $\sqrt{\frac{1+\beta}{1-\beta}}$.

## Part 3

* The speed $u$ of the flashlight in $F$ must be such that: $\sqrt{\frac{1+\beta_u}{1-\beta_u}}=\sqrt{\frac{1+\beta_{u'}}{1-\beta_{u'}}}\sqrt{\frac{1+\beta_v}{1-\beta_v}}$!
* We have an equation relating $u$ to $v$ and $u'$. If we solve for $u$, we're done!

## Part 4

* Square both sides and multiply the top and bottom of every fraction by $c$:
* $\frac{c+u}{c-u}=\frac{c+u'}{c-u'}\frac{c+v}{c-v}$.
* Let's solve for $u$.

## Part 4

$$
\begin{align*}
\frac{c+u}{c-u}&=\frac{c+u'}{c-u'}\frac{c+v}{c-v}\\
\class{fragment}{(c+u)(c-u')(c-v)}&\class{fragment}{{}=(c-u)(c+u')(c+v)}\\
\end{align*}
$$

$$
\begin{align*}
&\class{fragment}{u((c-u')(c-v)+(c+u')(c+v))}\\&\class{fragment}{{}=c((c+u')(c+v)-(c-u')(c-v))}
\end{align*}
$$

## Part 4

* Now:

$$
\begin{align*}
\class{fragment}{(c+u')(c+v)}&\class{fragment}{{}=c^2+c(u'+v)+u'v}\\
\class{fragment}{(c-u')(c-v)}&\class{fragment}{{}=c^2-c(u'+v)+u'v}\\
\class{fragment}{{}(c+u')(c+v)+(c+u')(c-v)}&\class{fragment}{{}=2(c^2+u'v)}\\
\class{fragment}{{}(c+u')(c+v)-(c+u')(c-v)}&\class{fragment}{{}=2c(u'+v)}\\
\end{align*}
$$

## Part 4

$$
\begin{align*}
\class{fragment}{u(2(c^2+u'v))}&\class{fragment}{{}=c(2c(u'+v))}\\
\class{fragment}{u}&\class{fragment}{{}=\frac{c^2(u'+v)}{c^2+u'v}}\\
&\class{fragment}{{}=\frac{u'+v}{1+\frac{u'v}{c^2}}}
\end{align*}
$$

## Result

* If $F'$ has velocity $v$ relative to $F$, and $F''$ has velocity $u'$ relative to $F'$, then the velocity of $F''$ relative to $F$ is $u=\frac{u'+v}{1+\frac{u'v}{c^2}}$.
* Equivalently, $\beta_u=\frac{\beta_{u'}+\beta_v}{1+\beta_{u'}\beta_v}$.

## Result

::: {.columns}
:::: {.column .fragment}

![Velocity Addition, Naive (source: me)](/images/5/velocity_addition_bad.png)

::::

:::: {.column .fragment}

![Velocity Addition, Actual (source: me)](/images/5/velocity_addition.png)

::::

:::

## Observations

* $F'$ is traveling at $v=0.9c$ relative to $F$. $F''$ is traveling at $u'=0.9c$ relative to $F'$. [What is the speed $u$ of $F''$ relative to $F$?]{.fragment}
* Naively: $u=u'+v=1.8c>c$ — bad!
* Actually: $u=\frac{u'+v}{1+\frac{u'v}{c^2}}=\frac{1.8c}{1+0.81}\approx 0.994c<c$ — good!

## Observations

* $F'$ is traveling at $v=100\,\textrm{m/s}$ relative to $F$. $F''$ is traveling at $u'=100\,\textrm{m/s}$ relative to $F'$. [What is the speed $u$ of $F''$ relative to $F$?]{.fragment}
* Naively: $u=u'+v=200\,\textrm{m/s}$.
* Actually: $u=\frac{u'+v}{1+\frac{u'v}{c^2}}=200\,\textrm{m/s}\class{fragment}{{}-2.225\times 10^{-11}\,\textrm{m/s}.}$


## Observations

* $F'$ emits a photon in the $+x$ direction. What is its speed $u$ relative to $F$?
	* Now, $u'=c$
* $u=\frac{c+v}{1+\frac{cv}{c^2}}=\frac{c^2(c+v)}{c^2+cv}=\frac{c^2(c+v)}{c(c+v)}=c$.&nbsp;
	* Phew! (It didn't matter what $v$ was.)

## Observations

* $F'$ emits a photon in the $-x$ direction. What is its speed $u$ relative to $F$?
	* Now, $u'=-c$
* $u=\frac{-c+v}{1+\frac{-cv}{c^2}}=\frac{c^2(-c+v)}{c^2-cv}=\frac{c^2(-c+v)}{c(c-v)}=-c$.&nbsp;
	* Phew! (It didn't matter what $v$ was.)

## Conclusion

* We can now deal with three (and, by repeating this process, arbitrarily many) frames in relative motion.
* The velocity addition formula handles both massive objects and photons equivalently.
* No amount of velocity addition can get something to appear to travel faster than light.
